rupicola/README.md
@@ -4,15 +4,17 @@ Next challenges:
 * Limitations of type classes
   - [ ] Pattern matching -- an inherent problem of F*, one cannot abstract over them anyway. Not a typeclass problem.
       	Typeclasses do not add any expressivity to F*. We're limited by what we can abstract away in F*.
-	For PMs, maybe one can generate instances on the fly.
-  - [ ] How powerful is phase1? A lot seems to get erased, which can be problematic if we want to claim any kind of end-to-end result.
-  - [ ] Typeclasses in F* may be less fancy than other languages. We expect it to be portable.
+	For PMs, maybe one can generate instances on the fly. There is another project requiring this.
+  - [ ] How powerful is phase1? A lot seems to happen, which can be problematic if we want to claim any kind of end-to-end result.
+        Typeclasses in F* may be less fancy than other languages. We expect it to be portable.
 * Features of Dependently Typed Languages:
-  - [ ] Compiling fixpoints (may work with F* if one defines instances for different arrities)
-  - [ ] Compiling Dependent Pairs/Functions
+  - [ ] Compiling fixpoints (may work with F* if one defines instances for different arrities). Stuck [FStarLang/FStar#3991](https://github.com/FStarLang/FStar/issues/3991)
+  - [x] Compiling pairs
+    - [ ] Automation problems when compiling fst / snd. [See here](https://github.com/andricicezar/fstar-io/blob/010dda6a013cb23288ad14019eca03b2bea2bdd0/rupicola/stlc_v2/Compiler.fst#L290).
+  - [ ] Compiling Dependent Pairs/Functions. See attempt on [dpair2](https://github.com/andricicezar/fstar-io/blob/dpairs2/rupicola/stlc_v2/Compiler.fst#L359) branch.
 * Features of F\*:
-  - [ ] WIP: Compiling refined types
-  - [ ] Dealing with pre-conditionality
+  - [x] Compiling refined types
+    - [ ] [Automation does not work when erasing](https://github.com/andricicezar/fstar-io/blob/010dda6a013cb23288ad14019eca03b2bea2bdd0/rupicola/refinements/Compiler.fst#L333)
   - [ ] Compiling arrows with pre-post-conditions
   - [ ] Compiling effects?
 * Compiling the identity monad
